theories/SemSound.v
@@ -168,17 +168,17 @@ Proof.
         sfirstorder.
       + qauto l: on.
   (* Par-R *)
-  - admit.
-    (* edestruct H as [A [B [C L]]]; eauto.
+  - 
+    edestruct H as [A [B [C L]]]; eauto.
     edestruct H0 as [A' [B' [C' L']]]; eauto.
     split; try split; try split.
     + sauto lq: on.
     + intros. sinvert H4. econstructor; eauto. sfirstorder.
     + sfirstorder.
-    + intros. rewrite -> H4 in *. edestruct i_ub_inert as [H00 H01]; eauto. rewrite H00 in *. rewrite H01 in *. sfirstorder. *)
+    + intros. rewrite -> H4 in *. edestruct i_ub_inert as [H00 H01]; eauto. rewrite H00 in *. rewrite H01 in *. sfirstorder.
   (* Cat-R-1 *)
-  - admit.
-    (* edestruct H as [A [B [C L]]]; eauto.
+  - 
+    edestruct H as [A [B [C L]]]; eauto.
     sinvert H1.
     sinvert H2.
     destruct H10;[|shelve].
@@ -190,10 +190,10 @@ Proof.
     Unshelve.
     assert (MaximalOn (fv e1) n). { eapply prop_on_contains. eapply typing_fv. eauto. eauto. }
     assert (MaximalPrefix p) by sauto lq: on.
-    best. *)
+    best.
   (* Cat-R-2 *)
-  - admit.
-    (* edestruct H as [A [B C]]; eauto.
+  - 
+    edestruct H as [A [B C]]; eauto.
     edestruct H0 as [A' [B' C']]; eauto.
     split; try split; try split.
     + hauto l: on.
@@ -206,10 +206,10 @@ Proof.
       assert (EmptyOn (fv e1) n) by hauto q: on use:prop_on_contains.
       assert (EmptyPrefix p1) by best.
       assert (Nullable s1) by best use:empty_and_maximal_means_nullable.
-      best. *)
+      best.
   (* Par-L *)
-  - admit.
-    (* assert (H00 : PrefixTyped (PfxParPair p1 p2) (TyPar s0 t)) by hauto l: on use: maps_to_has_type_reflect.
+  - 
+    assert (H00 : PrefixTyped (PfxParPair p1 p2) (TyPar s0 t)) by hauto l: on use: maps_to_has_type_reflect.
     sinvert H00. edestruct H as [A [B C]].
     + sfirstorder.
     + eassumption.
@@ -229,10 +229,10 @@ Proof.
            intro test. cbn. destruct (eqb_spec x test); destruct (eqb_spec y test); sfirstorder.
         -- econstructor; [| | | eauto | eauto |]. eauto. hauto q:on drew:off use:fv_hole_derivative. hauto q:on drew:off use:fv_hole_derivative. eapply B; eauto.
       * intros. eapply C. admit.
-      * intros H00 H01. admit. *)
+      * intros H00 H01. admit.
   (* cat-l-1 *)
-  - admit.
-    (*assert (H00 : PrefixTyped (PfxCatFst p) (TyDot s0 t)) by best use:maps_to_has_type_reflect.
+  - 
+    assert (H00 : PrefixTyped (PfxCatFst p) (TyDot s0 t)) by best use:maps_to_has_type_reflect.
     sinvert H00. edestruct H as [A [B C]]. eauto. eauto. eauto. eapply catrenvtyped1; eauto.
     assert (DisjointSets (dom (singleton_env x p)) (dom (singleton_env y (emp t)))). { eapply DisjointSets_inj. intros x0 H00. intro H01. eapply dom_singleton in H00. eapply dom_singleton in H01. scongruence. }
     assert (DisjointSets (dom (env_union (singleton_env x p) (singleton_env y (emp t)))) (fv G)). { eapply DisjointSets_inj. intros x0 H00. intro H01. eapply dom_union in H00. destruct H00; eapply dom_singleton in H10; scongruence. }
@@ -246,10 +246,9 @@ Proof.
       econstructor; [ eauto | eauto | eauto | | | eauto | | ]. hauto q: on use:fv_hole_derivative. hauto q: on use:fv_hole_derivative. eauto.
       hauto l: on.
     + eapply preserves_cat_1; eauto.
-    *)
   (* cat-l-2 *)
-  - admit.
-    (*assert (H00 : PrefixTyped (PfxCatBoth p1 p2) (TyDot s0 t)) by best use:maps_to_has_type_reflect.
+  - 
+    assert (H00 : PrefixTyped (PfxCatBoth p1 p2) (TyDot s0 t)) by best use:maps_to_has_type_reflect.
     sinvert H00. edestruct H as [A [B C]]. eauto. eauto. eauto. eapply catrenvtyped2; eauto.
     split; try split.
     + sfirstorder.
@@ -274,10 +273,9 @@ Proof.
         { eapply hole_compose_fill. eapply reflect_hole_compose; eauto. exists (CtxSemic CtxEmpty (CtxHasTy z s'0)). split. hauto l:on. scongruence use:reflect_fill. }
         eapply (typing_subst (hole_compose G' (HoleSemicR (CtxHasTy x s'') HoleHere))). eauto. { eapply context_derivative_wf; [|eauto]; eauto. } { intro H00. eapply hole_compose_fv_fn in H00. destruct H00. eapply fv_hole_derivative in H20;[|eauto]. sfirstorder. sfirstorder. } { eapply (hole_compose_fill G' ((HoleSemicR (CtxHasTy x s'') HoleHere))). hauto l:on use:reflect_hole_compose. exists (CtxSemic (CtxHasTy x s'') (CtxHasTy y s'0)). sfirstorder. } { eapply (hole_compose_fill G' ((HoleSemicR (CtxHasTy x s'') HoleHere))). hauto l: on use:reflect_hole_compose. exists (CtxSemic (CtxHasTy x s'') (CtxHasTy z s'0)). split; best use:reflect_fill. }
     + eapply preserves_cat_2; eauto.
-    *)
   (* Let *)
-  - admit.
-    (*edestruct H as [A [B [U V]]]; eauto.
+  - 
+    edestruct H as [A [B [U V]]]; eauto.
    (* todo: need better automation for disjoitnness *)
     assert (NoConflictOn eta (singleton_env x p) (fv G)). { eapply no_conflict_on_disjoint. right. eapply DisjointSets_inj. intros. intro. assert (x0 <> x) by scongruence. assert (x = x0) by qauto l: on use:dom_singleton. sfirstorder. }
     assert (EnvTyped (env_subst x p eta) Gxs). eapply env_subctx_bind'; [ | eauto | eauto | | | ]. eauto. eauto. { eapply env_typed_singleton. eauto. } { eapply preserves_to_agree. eapply typing_fv; eauto. sfirstorder. }
@@ -289,7 +287,7 @@ Proof.
     + intros GD' t'. intros.
       edestruct (fill_derivative eta G D GD GD') as [G' [D' [L [M [N O]]]]]; eauto.
       edestruct (derivative_fun p) as [s']; eauto.
-      assert (Typed D' NoRec e1' s' Inert) by hauto l: on.
+      assert (Typed nil D' NoRec e1' s' Inert) by hauto l: on.
       edestruct (O (CtxHasTy x s1) (CtxHasTy x s') Gxs (singleton_env x p)) as [G'xs' [W X]]. eauto. eauto. hauto l: on.
       econstructor; [ | eauto | | eauto | ]. hauto q:on use:fv_hole_derivative. eauto.
       eapply B'; eauto. 
@@ -297,10 +295,9 @@ Proof.
       eapply U'. eapply prop_on_minus. eapply U. hauto q: on. eauto.
     + intros. assert (EmptyOn (set_minus (fv e2) (singleton_set x)) eta) by hauto q: on.
       eapply V'. eauto. eapply prop_on_minus. eapply V. eauto. hauto q: on. eauto.
-      *)
   (* sum-l-1 *)
-  - admit.
-    (*split; try split; try split.
+  - 
+    split; try split; try split.
     + best use:emp_well_typed.
     + intros.
       assert (Derivative (emp r) r r) by best use:derivative_emp.
@@ -314,10 +311,9 @@ Proof.
       assert (Hcontra : MaximalPrefix PfxSumEmp) by qauto l:on.
       sinvert Hcontra.
     + best use:emp_empty.
-    *)
   (* sum-l-2 *)
-  - admit.
-    (*assert (WFContext Gz) by sfirstorder use:context_derivative_wf'.
+  - 
+    assert (WFContext Gz) by sfirstorder use:context_derivative_wf'.
     assert (Hwf : WFHole G /\ DisjointSets (fv G) (singleton_set z)) by sauto use:wf_fill_reflect.
     destruct Hwf.
     assert (~ fv G z) by sfirstorder.
@@ -357,10 +353,9 @@ Proof.
       edestruct (H02 z) as [p'' [UU UU']]; eauto.
       destruct (ltac:(scongruence) : PfxSumInl p = p'').
       sinvert UU'.
-      *)
   (* sum-l-3 *)
-  - admit.
-    (*assert (WFContext Gz) by sfirstorder use:context_derivative_wf'.
+  - 
+    assert (WFContext Gz) by sfirstorder use:context_derivative_wf'.
     assert (Hwf : WFHole G /\ DisjointSets (fv G) (singleton_set z)) by sauto use:wf_fill_reflect.
     destruct Hwf.
     assert (~ fv G z) by sfirstorder.
@@ -402,7 +397,6 @@ Proof.
       edestruct (H02 z) as [p'' [UU UU']]; eauto.
       destruct (ltac:(scongruence) : PfxSumInr p = p'').
       sinvert UU'.
-    *)
   (* fix *)
   - edestruct H as [A [B [[U V] [D E]]]]; eauto.
     assert (Typed nil g NoRec (histval_subst_all vs (fix_subst g r e e)) r i). eapply typing_histval_subst_all. { eapply typing_fix_subst; eauto. } { eapply HistArgsStep_sound; eauto. }
