theories/Subst.v
@@ -37,13 +37,14 @@ Fixpoint subst_var (e : term) (x : string) (y : string) : term :=
   | TmInr e =>
       TmInr (subst_var e x y)
   | TmPlusCase eta r z x' e1 y' e2 =>
-      TmPlusCase eta r z x' (subst_var e1 x y) y' (subst_var e2 x y)
+      TmPlusCase eta r (subst_str x y z) x' (subst_var e1 x y) y' (subst_var e2 x y)
   | TmFix args hpargs g r e =>
       TmFix (subst_var_argsterm args x y) hpargs g r e
   | TmRec args hpargs =>
       TmRec (subst_var_argsterm args x y) hpargs
   | TmArgsLet args g e => TmArgsLet (subst_var_argsterm args x y) g e
   | TmHistPgm hp r' => TmHistPgm hp r'
+  | TmWait eta r' s' z e => TmWait eta r' s' (subst_str x y z) (subst_var e x y)
   end
 with subst_var_argsterm (args : argsterm) (x : string) (y : string) :=
   match args with
